loop.ml
@@ -1,0 +1,30 @@
+needs "Library/iter.ml";;
+
+let LOOP = new_definition
+  `LOOP N B = \x y. ~B y /\ x = N y`;;
+
+(*
+search [`WF(<)`] (* WF_num *)
+search [`x ==> WF(y)`]
+*)
+
+let MINIMAL_SUC = prove
+  (`!P. (?n. P n) /\ ~(P 0) ==> (minimal) P = SUC ((minimal) (P o SUC))`,
+   GEN_TAC THEN SUBST1_TAC (MESON [num_CASES; NOT_SUC]
+       `(?n. P n) /\ ~(P 0) <=> (?n. (P (SUC n))) /\ ~(P 0)`) THEN
+   REWRITE_TAC[REWRITE_RULE[o_THM] (SPEC `(P:num->bool) o SUC` MINIMAL)] THEN
+   STRIP_TAC THEN MATCH_MP_TAC MINIMAL_UNIQUE THEN CONJ_TAC THENL
+   [FIRST_ASSUM ACCEPT_TAC; ALL_TAC] THEN
+   GEN_TAC THEN DISJ_CASES_TAC (SPEC `m:num` num_CASES) THEN
+   ASM_REWRITE_TAC[] THEN POP_ASSUM (CHOOSE_THEN SUBST1_TAC) THEN
+   ASM_SIMP_TAC[LT_SUC]);;
+
+let WF_LOOP = prove
+  (`!N (B:A->bool). (!s. ~B s ==> ?n. B (ITER n N s)) ==> WF(LOOP N B)`,
+   REPEAT STRIP_TAC THEN MATCH_MP_TAC WF_SUBSET THEN
+   EXISTS_TAC `MEASURE (\s. minimal n. (B:A->bool) (ITER n N s))` THEN
+   REWRITE_TAC[WF_MEASURE; MEASURE; LOOP] THEN REPEAT STRIP_TAC THEN
+   POP_ASSUM SUBST1_TAC THEN REWRITE_TAC[GSYM ITER_ALT] THEN
+   MP_TAC(SPEC `\n. (B:A->bool) (ITER n N y)` MINIMAL_SUC) THEN
+   ASM_SIMP_TAC[CONJUNCT1 ITER; o_DEF] THEN DISCH_THEN SUBST1_TAC THEN
+   REWRITE_TAC[LT]);;
